# baseURI: https://brickschema.org/schema/Brick
# imports: http://datashapes.org/dash
# prefix: brick

@prefix brick: <https://brickschema.org/schema/Brick#> .
@prefix dash: <http://datashapes.org/dash#> .
@prefix owl: <http://www.w3.org/2002/07/owl#> .
@prefix quantitykind: <http://qudt.org/vocab/quantitykind/> .
@prefix rdf: <http://www.w3.org/1999/02/22-rdf-syntax-ns#> .
@prefix rdfs: <http://www.w3.org/2000/01/rdf-schema#> .
@prefix sh: <http://www.w3.org/ns/shacl#> .
@prefix unit: <http://qudt.org/vocab/unit/> .
@prefix xsd: <http://www.w3.org/2001/XMLSchema#> .

<https://brickschema.org/schema/Brick>
  a owl:Ontology ;
  rdfs:comment "This is a proxy stub for a future Brick 2 based on SHACL shapes, for integration testing with a future REC 4 also based on SHACL shapes. We make no guarantees as to whether this is the direction either project will actually take; this early prototype level stuff." ;
  rdfs:label "Brick Schema stub" ;
  owl:imports <http://datashapes.org/dash> ;
  owl:versionInfo "2.0" ;
.
brick:Alarm
  a rdfs:Class ;
  a sh:NodeShape ;
  rdfs:comment "Alarm points are signals (either audible or visual) that alert an operator to an off-normal condition which requires some form of corrective action." ;
  rdfs:label "Alarm" ;
  rdfs:subClassOf brick:Point ;
.
brick:Camera
  a rdfs:Class ;
  a sh:NodeShape ;
  rdfs:label "Camera" ;
  rdfs:subClassOf brick:Equipment ;
.
brick:Command
  a rdfs:Class ;
  a sh:NodeShape ;
  rdfs:comment "A Command is an output point that directly determines the behavior of equipment and/or affects relevant operational points." ;
  rdfs:label "Command" ;
  rdfs:subClassOf brick:Point ;
.
brick:DurationSensor
  a rdfs:Class ;
  a sh:NodeShape ;
  rdfs:label "Duration sensor" ;
  rdfs:subClassOf brick:Sensor ;
  sh:property [
      a sh:PropertyShape ;
      sh:path brick:value ;
      sh:datatype xsd:duration ;
      sh:maxCount 1 ;
      sh:name "value" ;
      sh:nodeKind sh:Literal ;
    ] ;
  sh:property [
      sh:path brick:measures ;
      sh:hasValue quantitykind:Time ;
      sh:maxCount 1 ;
    ] ;
.
brick:Equipment
  a rdfs:Class ;
  a sh:NodeShape ;
  rdfs:comment "Devices that serve all or part of the building and may include electric power, lighting, transportation, or service water heating, including, but not limited to, furnaces, boilers, air conditioners, heat pumps, chillers, water heaters, lamps, luminaires, ballasts, elevators, escalators, or other devices or installations." ;
  rdfs:label "Equipment" ;
.
brick:Meter
  a rdfs:Class ;
  a sh:NodeShape ;
  rdfs:comment "A device that measure usage or consumption of some media --- typically a form energy or power." ;
  rdfs:label "Meter" ;
  rdfs:subClassOf brick:Equipment ;
.
brick:Motor
  a rdfs:Class ;
  a sh:NodeShape ;
  rdfs:comment "A machine in which power is applied to do work by the conversion of various forms of energy into mechanical force and motion." ;
  rdfs:label "Motor" ;
  rdfs:subClassOf brick:Equipment ;
.
brick:Parameter
  a rdfs:Class ;
  a sh:NodeShape ;
  rdfs:comment "Parameter points are configuration settings used to guide the operation of equipment and control systems; for example they may provide bounds on valid setpoint values." ;
  rdfs:label "Parameter" ;
  rdfs:subClassOf brick:Point ;
.
brick:Point
  a rdfs:Class ;
  a sh:NodeShape ;
  rdfs:label "Point" ;
  rdfs:subClassOf rdfs:Resource ;
  sh:property [
      a sh:PropertyShape ;
      sh:path brick:value ;
      sh:maxCount 1 ;
      sh:name "value" ;
      sh:nodeKind sh:Literal ;
    ] ;
.
brick:Sensor
  a rdfs:Class ;
  a sh:NodeShape ;
  rdfs:comment "A Sensor is an input point that represents the value of a device or instrument designed to detect and measure a variable (ASHRAE Dictionary)." ;
  rdfs:label "Sensor" ;
  rdfs:subClassOf brick:Point ;
.
brick:Setpoint
  a rdfs:Class ;
  a sh:NodeShape ;
  rdfs:comment "A Setpoint is an input value at which the desired property is set." ;
  rdfs:label "Setpoint" ;
  rdfs:subClassOf brick:Point ;
.
brick:Status
  a rdfs:Class ;
  a sh:NodeShape ;
  rdfs:comment "A Status is input point that reports the current operating mode, state, position, or condition of an item. Statuses are observations and should be considered 'read-only'." ;
  rdfs:label "Status" ;
  rdfs:subClassOf brick:Point ;
.
brick:TemperatureSensor
  a rdfs:Class ;
  a sh:NodeShape ;
  rdfs:comment "Measures temperature: the physical property of matter that quantitatively expresses the common notions of hot and cold." ;
  rdfs:label "Temperature sensor" ;
  rdfs:subClassOf brick:Sensor ;
  sh:property [
      a sh:PropertyShape ;
      sh:path brick:unit ;
      sh:in (
          unit:DEG_C
          unit:DEG_F
        ) ;
      sh:maxCount 1 ;
      sh:name "unit" ;
    ] ;
  sh:property [
      a sh:PropertyShape ;
      sh:path brick:value ;
      sh:datatype xsd:decimal ;
      sh:maxCount 1 ;
      sh:name "value" ;
    ] ;
  sh:property [
      sh:path brick:measures ;
      sh:hasValue quantitykind:Temperature ;
      sh:maxCount 1 ;
      sh:name "measures" ;
    ] ;
.
brick:Valve
  a rdfs:Class ;
  a sh:NodeShape ;
  rdfs:comment "A device that regulates, directs or controls the flow of a fluid by opening, closing or partially obstructing various passageways." ;
  rdfs:label "Valve" ;
  rdfs:subClassOf brick:Equipment ;
.
