# baseURI: https://w3id.org/rec/breck
# imports: http://datashapes.org/dash

@prefix brick: <https://brickschema.org/schema/Brick#> .
@prefix dash: <http://datashapes.org/dash#> .
@prefix owl: <http://www.w3.org/2002/07/owl#> .
@prefix quantitykind: <http://qudt.org/vocab/quantitykind/> .
@prefix rdf: <http://www.w3.org/1999/02/22-rdf-syntax-ns#> .
@prefix rdfs: <http://www.w3.org/2000/01/rdf-schema#> .
@prefix rec: <https://w3id.org/rec#> .
@prefix sh: <http://www.w3.org/ns/shacl#> .
@prefix unit: <http://qudt.org/vocab/unit/> .
@prefix xsd: <http://www.w3.org/2001/XMLSchema#> .

<https://brickschema.org/schema/Brick>
  rdfs:comment "This is a proxy stub for a future Brick 2 based on SHACL shapes, for integration testing with a future REC 4 also based on SHACL shapes. We make no guarantees as to whether this is the direction either project will actually take; this early prototype level stuff." ;
  rdfs:label "Brick Schema stub" ;
  owl:versionInfo "2.0" ;
.
brick:Alarm
  a rdfs:Class ;
  a sh:NodeShape ;
  rdfs:comment "Alarm points are signals (either audible or visual) that alert an operator to an off-normal condition which requires some form of corrective action." ;
  rdfs:label "Alarm" ;
  rdfs:subClassOf brick:Point ;
.
brick:Camera
  a rdfs:Class ;
  a sh:NodeShape ;
  rdfs:label "Camera" ;
  rdfs:subClassOf brick:Equipment ;
.
brick:Command
  a rdfs:Class ;
  a sh:NodeShape ;
  rdfs:comment "A Command is an output point that directly determines the behavior of equipment and/or affects relevant operational points." ;
  rdfs:label "Command" ;
  rdfs:subClassOf brick:Point ;
.
brick:DurationSensor
  a rdfs:Class ;
  a sh:NodeShape ;
  rdfs:label "Duration sensor" ;
  rdfs:subClassOf brick:Sensor ;
  sh:property [
      a sh:PropertyShape ;
      sh:path brick:value ;
      sh:datatype xsd:duration ;
      sh:maxCount 1 ;
      sh:name "value" ;
      sh:nodeKind sh:Literal ;
    ] ;
  sh:property [
      sh:path brick:measures ;
      sh:hasValue quantitykind:Time ;
      sh:maxCount 1 ;
    ] ;
.
brick:Equipment
  a rdfs:Class ;
  a sh:NodeShape ;
  rdfs:comment "Devices that serve all or part of the building and may include electric power, lighting, transportation, or service water heating, including, but not limited to, furnaces, boilers, air conditioners, heat pumps, chillers, water heaters, lamps, luminaires, ballasts, elevators, escalators, or other devices or installations." ;
  rdfs:label "Equipment" ;
  rdfs:subClassOf rec:Asset ;
  sh:property [
      a sh:PropertyShape ;
      sh:path brick:hasPoint ;
      sh:class brick:Point ;
      sh:name "has point" ;
      sh:nodeKind sh:IRI ;
    ] ;
.
brick:Meter
  a rdfs:Class ;
  a sh:NodeShape ;
  rdfs:comment "A device that measure usage or consumption of some media --- typically a form energy or power." ;
  rdfs:label "Meter" ;
  rdfs:subClassOf brick:Equipment ;
.
brick:Motor
  a rdfs:Class ;
  a sh:NodeShape ;
  rdfs:comment "A machine in which power is applied to do work by the conversion of various forms of energy into mechanical force and motion." ;
  rdfs:label "Motor" ;
  rdfs:subClassOf brick:Equipment ;
.
brick:Parameter
  a rdfs:Class ;
  a sh:NodeShape ;
  rdfs:comment "Parameter points are configuration settings used to guide the operation of equipment and control systems; for example they may provide bounds on valid setpoint values." ;
  rdfs:label "Parameter" ;
  rdfs:subClassOf brick:Point ;
.
brick:Point
  a rdfs:Class ;
  a sh:NodeShape ;
  rdfs:label "Point" ;
  rdfs:subClassOf rdfs:Resource ;
  sh:property [
      a sh:PropertyShape ;
      sh:path brick:value ;
      sh:maxCount 1 ;
      sh:name "value" ;
      sh:nodeKind sh:Literal ;
    ] ;
.
brick:Sensor
  a rdfs:Class ;
  a sh:NodeShape ;
  rdfs:comment "A Sensor is an input point that represents the value of a device or instrument designed to detect and measure a variable (ASHRAE Dictionary)." ;
  rdfs:label "Sensor" ;
  rdfs:subClassOf brick:Point ;
.
brick:Setpoint
  a rdfs:Class ;
  a sh:NodeShape ;
  rdfs:comment "A Setpoint is an input value at which the desired property is set." ;
  rdfs:label "Setpoint" ;
  rdfs:subClassOf brick:Point ;
.
brick:Status
  a rdfs:Class ;
  a sh:NodeShape ;
  rdfs:comment "A Status is input point that reports the current operating mode, state, position, or condition of an item. Statuses are observations and should be considered 'read-only'." ;
  rdfs:label "Status" ;
  rdfs:subClassOf brick:Point ;
.
brick:TemperatureSensor
  a rdfs:Class ;
  a sh:NodeShape ;
  rdfs:comment "Measures temperature: the physical property of matter that quantitatively expresses the common notions of hot and cold." ;
  rdfs:label "Temperature sensor" ;
  rdfs:subClassOf brick:Sensor ;
  sh:property [
      a sh:PropertyShape ;
      sh:path brick:unit ;
      sh:in (
          unit:DEG_C
          unit:DEG_F
        ) ;
      sh:maxCount 1 ;
      sh:name "unit" ;
    ] ;
  sh:property [
      a sh:PropertyShape ;
      sh:path brick:value ;
      sh:datatype xsd:decimal ;
      sh:maxCount 1 ;
      sh:name "value" ;
    ] ;
  sh:property [
      sh:path brick:measures ;
      sh:hasValue quantitykind:Temperature ;
      sh:maxCount 1 ;
      sh:name "measures" ;
    ] ;
.
brick:Valve
  a rdfs:Class ;
  a sh:NodeShape ;
  rdfs:comment "A device that regulates, directs or controls the flow of a fluid by opening, closing or partially obstructing various passageways." ;
  rdfs:label "Valve" ;
  rdfs:subClassOf brick:Equipment ;
.
<https://w3id.org/rec>
  rdfs:label "RealEstateCore" ;
  owl:versionInfo "4.0" ;
.
rec:Agent
  a rdfs:Class ;
  a sh:NodeShape ;
  rdfs:comment "The human, group, or machine that consumes or acts upon an object or data. This higher-level grouping allows properties that are shared among its subclasses (Person, Organization, ....) to be anchored in one joint place, on the Agent class." ;
  rdfs:label "Agent" ;
  rdfs:subClassOf rdfs:Resource ;
  sh:property [
      a sh:PropertyShape ;
      sh:path rec:memberOf ;
      sh:class rec:Organization ;
      sh:name "member of" ;
      sh:nodeKind sh:IRI ;
    ] ;
  sh:property [
      a sh:PropertyShape ;
      sh:path rec:name ;
      sh:datatype xsd:string ;
      sh:name "name" ;
    ] ;
.
rec:Apartment
  a rdfs:Class ;
  a sh:NodeShape ;
  rdfs:label "Apartment" ;
  rdfs:subClassOf rec:Collection ;
  sh:property [
      a sh:PropertyShape ;
      sh:path rec:includes ;
      sh:class rec:Room ;
      sh:minCount 1 ;
      sh:name "includes" ;
      sh:nodeKind sh:IRI ;
    ] ;
.
rec:Architecture
  a rdfs:Class ;
  a sh:NodeShape ;
  rdfs:comment "A designed/landscaped (or potentially designed/landscaped) part of the physical world that has a 3D spatial extent. E.g., a building site, a building, levels within the building, rooms, etc." ;
  rdfs:label "Architecture" ;
  rdfs:subClassOf rec:Space ;
  sh:property [
      a sh:PropertyShape ;
      sh:path brick:hasPoint ;
      sh:class brick:Point ;
      sh:name "has point" ;
      sh:nodeKind sh:IRI ;
    ] ;
  sh:property [
      a sh:PropertyShape ;
      sh:path rec:address ;
      sh:class rec:PostalAddress ;
      sh:description "Physical address of the architecture (site, building, sub-building, entrance room, etc.) in question." ;
      sh:name "address" ;
      sh:nodeKind sh:IRI ;
    ] ;
  sh:property [
      a sh:PropertyShape ;
      sh:path rec:adjacentElement ;
      sh:class rec:BuildingElement ;
      sh:name "adjacent element" ;
      sh:nodeKind sh:IRI ;
    ] ;
  sh:property [
      a sh:PropertyShape ;
      sh:path rec:architectedBy ;
      sh:class rec:Agent ;
      sh:name "architected by" ;
      sh:nodeKind sh:IRI ;
    ] ;
  sh:property [
      a sh:PropertyShape ;
      sh:path rec:constructedBy ;
      sh:class rec:Agent ;
      sh:nodeKind sh:IRI ;
    ] ;
  sh:property [
      a sh:PropertyShape ;
      sh:path rec:containsElement ;
      sh:class rec:BuildingElement ;
      sh:description "Links an Architecture to BuildingElement that is contained in the Space." ;
      sh:name "contains element" ;
      sh:nodeKind sh:IRI ;
    ] ;
  sh:property [
      a sh:PropertyShape ;
      sh:path rec:containsSpace ;
      sh:class rec:Architecture ;
      sh:name "contains space" ;
      sh:nodeKind sh:IRI ;
    ] ;
  sh:property [
      a sh:PropertyShape ;
      sh:path rec:intersectingElement ;
      sh:class rec:BuildingElement ;
      sh:name "intersecting element" ;
      sh:nodeKind sh:IRI ;
    ] ;
  sh:property [
      a sh:PropertyShape ;
      sh:path rec:operatedBy ;
      sh:class rec:Agent ;
      sh:name "operated by" ;
      sh:nodeKind sh:IRI ;
    ] ;
  sh:property [
      a sh:PropertyShape ;
      sh:path rec:ownedBy ;
      sh:class rec:Agent ;
      sh:name "owned by" ;
      sh:nodeKind sh:IRI ;
    ] ;
  sh:property [
      a sh:PropertyShape ;
      sh:path rec:subjectOf ;
      sh:class rec:Document ;
      sh:name "subject of" ;
      sh:nodeKind sh:IRI ;
    ] ;
.
rec:Asset
  a rdfs:Class ;
  a sh:NodeShape ;
  rdfs:comment "Something which is placed inside of a building, but is not an integral part of that building's structure; e.g., furniture, equipment, systems, etc." ;
  rdfs:label "Asset" ;
  rdfs:subClassOf rdfs:Resource ;
.
rec:BasementLevel
  a rdfs:Class ;
  a sh:NodeShape ;
  rdfs:label "Basement level" ;
  rdfs:subClassOf rec:Level ;
.
rec:Building
  a rdfs:Class ;
  a sh:NodeShape ;
  rdfs:comment "A confined building structure." ;
  rdfs:label "Building" ;
  rdfs:subClassOf rec:Architecture ;
.
rec:BuildingElement
  a rdfs:Class ;
  a sh:NodeShape ;
  rdfs:comment "A part that constitutes a piece of a building's structural makeup. E.g., Facade, Wall, Slab, RoofInner, etc." ;
  rdfs:label "Building element" ;
  rdfs:subClassOf rdfs:Resource ;
.
rec:Campus
  a rdfs:Class ;
  a sh:NodeShape ;
  rdfs:comment "A campus represents a collection of location entities. The constituent locations may have differing legal ownership and utilization purposes, but they are generally perceived as a coherent unit or sub-region within a city or other region. E.g., a university campus, a hospital campus, a corporate campus, etc." ;
  rdfs:label "Campus" ;
  rdfs:subClassOf rec:Collection ;
  sh:property [
      a sh:PropertyShape ;
      sh:path rec:includes ;
      sh:class rec:Architecture ;
      sh:minCount 1 ;
      sh:name "includes" ;
      sh:nodeKind sh:IRI ;
    ] ;
.
rec:Collection
  a rdfs:Class ;
  a sh:NodeShape ;
  rdfs:comment "An administrative grouping of entities that are adressed and treated as a unit for some purpose. These entities may have some spatial arrangement (e.g., an apartment is typically contiguous) but that is not a requirement (see, e.g., a distributed campus consisting of spatially disjoint plots or buildings)." ;
  rdfs:label "Collection" ;
  rdfs:subClassOf rdfs:Resource ;
.
rec:Document
  a rdfs:Class ;
  a sh:NodeShape ;
  rdfs:label "Document" ;
  rdfs:subClassOf rec:Information ;
  sh:property [
      a sh:PropertyShape ;
      sh:path rec:url ;
      sh:name "URL" ;
      sh:nodeKind sh:IRI ;
    ] ;
.
rec:Furniture
  a rdfs:Class ;
  a sh:NodeShape ;
  rdfs:label "Furniture" ;
  rdfs:subClassOf rec:Asset ;
.
rec:HVACZone
  a rdfs:Class ;
  a sh:NodeShape ;
  rdfs:label "HVAC zone" ;
  rdfs:subClassOf rec:Zone ;
.
rec:Information
  a rdfs:Class ;
  a sh:NodeShape ;
  rdfs:label "Information" ;
  rdfs:subClassOf rdfs:Resource ;
.
rec:Level
  a rdfs:Class ;
  a sh:NodeShape ;
  rdfs:comment "The level of a building, a.k.a. storey, floor, etc." ;
  rdfs:label "Level" ;
  rdfs:subClassOf rec:Architecture ;
  sh:property [
      a sh:PropertyShape ;
      sh:path rec:levelNumber ;
      sh:datatype xsd:integer ;
      sh:name "level number" ;
    ] ;
.
rec:MezzanineLevel
  a rdfs:Class ;
  a sh:NodeShape ;
  rdfs:label "Mezzanine level" ;
  rdfs:subClassOf rec:Level ;
.
rec:OccupancyZone
  a rdfs:Class ;
  a sh:NodeShape ;
  rdfs:label "Occupancy zone" ;
  rdfs:subClassOf rec:Zone ;
.
rec:Organization
  a rdfs:Class ;
  a sh:NodeShape ;
  rdfs:comment "An organization of any sort (e.g., a business, association, project, consortium, tribe, etc.)" ;
  rdfs:label "Organization" ;
  rdfs:subClassOf rec:Agent ;
  sh:property [
      a sh:PropertyShape ;
      sh:path rec:departmentOf ;
      sh:class rec:Organization ;
      sh:description "A relationship between a child organization and the parent organization that the child is a department of." ;
      sh:name "department of" ;
      sh:nodeKind sh:IRI ;
    ] ;
.
rec:Person
  a rdfs:Class ;
  a sh:NodeShape ;
  rdfs:comment "A natural person (i.e., an individual human being)." ;
  rdfs:label "Person" ;
  rdfs:subClassOf rec:Agent ;
  sh:property [
      a sh:PropertyShape ;
      sh:path rec:familyName ;
      sh:datatype xsd:string ;
    ] ;
  sh:property [
      a sh:PropertyShape ;
      sh:path rec:givenName ;
      sh:datatype xsd:string ;
    ] ;
.
rec:PostalAddress
  a rdfs:Class ;
  a sh:NodeShape ;
  rdfs:label "Postal address" ;
  rdfs:subClassOf rec:Information ;
  sh:property [
      a sh:PropertyShape ;
      sh:path rec:country ;
      sh:datatype xsd:string ;
      sh:description "The country, e.g., USA, Sweden, Argentina, or optionally a two-letter ISO 3166-1 alpha-2 country code, e.g., \"SE\", \"US\", etc." ;
      sh:maxCount 1 ;
      sh:name "country" ;
    ] ;
.
rec:Region
  a rdfs:Class ;
  a sh:NodeShape ;
  rdfs:comment "An administrative geospatial unit larger than the individual real estate. For instance, \"Lombary\", \"North America\", \"The Back Bay\", \"Elnätsområde Syd\", etc." ;
  rdfs:label "Region" ;
  rdfs:subClassOf rec:Space ;
.
rec:Roof
  a rdfs:Class ;
  a sh:NodeShape ;
  rdfs:label "Roof" ;
  rdfs:subClassOf rec:BuildingElement ;
.
rec:RoofLevel
  a rdfs:Class ;
  a sh:NodeShape ;
  rdfs:label "Roof level" ;
  rdfs:subClassOf rec:Level ;
.
rec:Room
  a rdfs:Class ;
  a sh:NodeShape ;
  rdfs:label "Room" ;
  rdfs:subClassOf rec:Architecture ;
.
rec:Site
  a rdfs:Class ;
  a sh:NodeShape ;
  rdfs:comment "A piece of land upon which zero or more buildings may be situated." ;
  rdfs:label "Site" ;
  rdfs:subClassOf rec:Architecture ;
.
rec:Slab
  a rdfs:Class ;
  a sh:NodeShape ;
  rdfs:label "Slab" ;
  rdfs:subClassOf rec:BuildingElement ;
.
rec:Space
  a rdfs:Class ;
  a sh:NodeShape ;
  rdfs:comment "A contiguous part of the physical world that contains or can contain sub-spaces. E.g., a Region can contain many Sites, which in turn can contain many Buildings." ;
  rdfs:label "Space" ;
  rdfs:subClassOf rdfs:Resource ;
  sh:property [
      a sh:PropertyShape ;
      sh:path rec:adjacentSpace ;
      sh:class rec:Space ;
      sh:name "adjacent space" ;
      sh:nodeKind sh:IRI ;
    ] ;
  sh:property [
      a sh:PropertyShape ;
      sh:path rec:containsSpace ;
      sh:class rec:Space ;
      sh:name "contains space" ;
      sh:nodeKind sh:IRI ;
    ] ;
  sh:property [
      a sh:PropertyShape ;
      sh:path rec:intersectingSpace ;
      sh:class rec:Space ;
      sh:name "intersecting space" ;
      sh:nodeKind sh:IRI ;
    ] ;
.
rec:Sub-building
  a rdfs:Class ;
  a sh:NodeShape ;
  rdfs:label "Sub-building" ;
  rdfs:subClassOf rec:Architecture ;
.
rec:Wall
  a rdfs:Class ;
  a sh:NodeShape ;
  rdfs:label "Wall" ;
  rdfs:subClassOf rec:BuildingElement ;
.
rec:Workspace
  a rdfs:Class ;
  a sh:NodeShape ;
  rdfs:label "Workspace" ;
  rdfs:subClassOf rec:Zone ;
.
rec:Zone
  a rdfs:Class ;
  a sh:NodeShape ;
  rdfs:comment "A sub-zone within a building defined to support some technology and/or use, e.g., an HVAC zone, a security zone, etc." ;
  rdfs:label "Zone" ;
  rdfs:subClassOf rec:Architecture ;
.
<https://w3id.org/rec/breck>
  a owl:Ontology ;
  owl:imports <http://datashapes.org/dash> ;
.
[
  a sh:PropertyShape ;
].
